\appendix
\appendixpage

\section{Proofs of Properties of Big-P Notation}

\subsection{Merging over Arithmetic Operations}
\label{MergingOverArithmetic}

\begin{theorem}
	$P$ merges over addition and subtraction. That is, for functions $f$ and $g$,
	\begin{align*}
	\hat{f} \TextTilde f \land \hat{g} \TextTilde g \rightarrow \begin{cases}
	(\hat{f} + \hat{g}) \TextTilde (f + g)\\
	(\hat{f} - \hat{g}) \TextTilde (f - g)
	\end{cases}
	\end{align*}
\end{theorem}

\begin{proof}
	We will consider the statement about addition first. Recall from the note at \ref{AsymptoticProperties} that this statement is equivalent to:
	
	\textit{Let $\hat{f} \in P(f(n))$ and $\hat{g} \in P(g(n))$. Then $\hat{f} + \hat{g} \in P(f(n) + g(n))$.}
	
	We can show this by using the limit definition of $P$. For brevity, we will omit the parameter $n$ to each function. Since
	
	\begin{align*}
	\lim_{n \to \infty} \left( \frac{\hat{f} + \hat{g}}{f + g} \right) &= \lim_{n \to \infty} \left( \frac{\hat{f}}{f + g} \right) + \lim_{n \to \infty} \left( \frac{\hat{g}}{f + g} \right)\\
	&= \left( \lim_{n \to \infty} \frac{\hat{f}}{f} \right) \left( \lim_{n \to \infty} \left( \frac{f}{f + g} \right) \right) +\\
	&\ \ \ \ \left( \lim_{n \to \infty} \frac{\hat{g}}{g} \right) \left( \lim_{n \to \infty} \left( \frac{g}{f + g} \right) \right)\\
	&= \lim_{n \to \infty} \left( \frac{f}{f + g} \right) + \lim_{n \to \infty} \left( \frac{g}{f + g} \right)\\
	&= \lim_{n \to \infty} \left( \frac{f + g}{f + g} \right)\\
	&= 1
	\end{align*}
	
	it follows that $\hat{f} + \hat{g} \in P(f(n) + g(n))$. The statement about subtraction can be proved in a similar fashion.
\end{proof}

\begin{theorem}
	$P$ merges over multiplication and division. That is, for functions $f$ and $g$,
	\begin{align*}
	\hat{f} \TextTilde f \land \hat{g} \TextTilde g \rightarrow \begin{cases}
	\hat{f}\hat{g} \TextTilde fg\\
	\hat{f} / \hat{g} \TextTilde f / g
	\end{cases}
	\end{align*}
\end{theorem}

\begin{proof}
	We will consider the statement about multiplication first. Recall from the note at \ref{AsymptoticProperties} that this statement is equivalent to:
	
	\textit{Let $\hat{f} \in P(f(n))$ and $\hat{g} \in P(g(n))$. Then $\hat{f}\hat{g} \in P(f(n)g(n))$.}
	
	We can show this easily by multiplying the limits corresponding to $\hat{f}$ and $\hat{g}$:
	
	\begin{align*}
	\lim_{n \to \infty} \frac{\hat{f}(n)}{f(n)} &= 1\\
	\lim_{n \to \infty} \frac{\hat{g}(n)}{g(n)} &= 1\\
	\left( \lim_{n \to \infty} \frac{\hat{f}(n)}{f(n)} \right) \left( \lim_{n \to \infty} \frac{\hat{g}(n)}{g(n)} \right) &= 1 \cdot 1\\
	\lim_{n \to \infty} \frac{\hat{f}(n)\hat{g}(n)}{f(n)g(n)} &= 1
	\end{align*}
	
	it follows that $\hat{f}\hat{g} \in P(f(n)g(n))$. The statement about division can be proved by flipping the fraction for $\hat{g}$ before multiplying, resulting in
	
	\begin{align*}
	\lim_{n \to \infty} \frac{\hat{f}(n) / \hat{g}(n)}{f(n) / g(n)} = 1
	\end{align*}
	
	This implies $\hat{f} / \hat{g} \in P(f(n) / g(n))$.
\end{proof}

\subsection{Unique Class Lemma}
\label{UniqueClassOfFunctions}

\begin{lemma}
	Each function $f(n)$ has a unique class of functions under $P$. That is, suppose $f \in P(g(n))$ and $f \in P(h(n))$. Then $P(g(n)) = P(h(n))$.
\end{lemma}

\begin{proof}
	By definition, $\lim_{n \to \infty} \frac{f(n)}{g(n)} = 1$ and $\lim_{n \to \infty} \frac{f(n)}{h(n)} = 1$. Flipping the first equation and multiplying, we receive
	
	\begin{align*}
	\left( \lim_{n \to \infty} \frac {g(n)} {f(n)} \right) \left( \lim_{n \to \infty} \frac {f(n)} {h(n)} \right) &= 1\\
	\lim_{n \to \infty} \frac {g(n)} {h(n)} &= 1\\
	g &\in P(h(n))
	\end{align*}
	
	Now, consider any $\hat{g} \in P(g(n))$. Since
	
	\begin{align*}
	\lim_{n \to \infty} \frac {\hat{g}(n)} {g(n)} &= 1\\
	\left( \lim_{n \to \infty} \frac {\hat{g}(n)} {g(n)} \right) \left( \lim_{n \to \infty} \frac{g(n)}{h(n)} \right) &= 1\\
	\lim_{n \to \infty} \frac{\hat{g}(n)}{h(n)} &= 1
	\end{align*}
	
	it follows that $\hat{g} \in P(h(n))$, and thus $P(g(n)) \subseteq P(h(n))$. By a similar argument, it can be shown $P(h(n)) \subseteq P(g(n))$. Thus it must be true that $P(g(n)) = P(h(n))$.
\end{proof}

\subsection{Removal of Lower-Order Terms}
\label{RemovesLowerOrderTerms}

\begin{theorem}
	If $\lim_{n \to \infty} \frac{g(n)}{f(n)} = 0$, then $P(f(n) + g(n)) = P(f(n))$.
\end{theorem}

\begin{proof}
	\begin{align*}
	\lim_{n \to \infty} \left( \frac{f(n) + g(n)}{f(n)} \right) &= \lim_{n \to \infty} \frac{f(n)}{f(n)} + \lim_{n \to \infty} \frac{g(n)}{f(n)}\\
	&= 1 + 0\\
	&= 1
	\end{align*}
	
	Then $f(n) + g(n) \in P(f(n))$. Since it is also true that $f(n) + g(n) \in P(f(n) + g(n))$, it follows from \ref{UniqueClassOfFunctions} that $P(f(n)) = P(f(n) + g(n))$.
\end{proof}